TM/Retract.v
@@ -1,5 +1,25 @@
 Require Import Shared.Base.
 
+Section Injection.
+
+  Variable X Y : Type.
+
+  Definition injective (f : X -> Y) := forall x1 x2, f x1 = f x2 -> x1 = x2.
+
+End Injection.
+
+Section Injection_Compose.
+  Variable X Y Z : Type.
+  Variable (f : X -> Y) (g : Y -> Z).
+  Hypothesis (f_inj : injective f) (g_inj : injective g).
+
+  Definition compose_inj : X -> Z := fun x => g (f x).
+
+  Lemma compose_inj_injective : injective compose_inj.
+  Proof. firstorder. Qed.
+End Injection_Compose.
+
+
 Section Retract.
 
   Variable X Y : Type.
@@ -21,10 +41,34 @@ Section Retract.
     intros x1 x2 H. enough (Some x1 = Some x2) as HE by now inv HE.
     erewrite <- !retract_g_adjoint; eauto. now rewrite H.
   Qed.
-
-  Definition retract_tight : Prop := forall x y, retract_g I y = Some x -> y = retract_f I x.
-
 End Retract.
+
+Section TightRetract.
+
+  Variable X Y : Type.
+
+  Record tight_retract :=
+    {
+      tretract_f : X -> Y;
+      tretract_g : Y -> option X;
+      tretract_inv : forall x y, tretract_g y = Some x <-> y = tretract_f x;
+    }.
+
+  Variable I : tight_retract.
+
+  Lemma tretract_g_adjoint : forall x, tretract_g I (tretract_f I x) = Some x.
+  Proof. intros. now apply tretract_inv. Qed.
+
+  Lemma tretract_g_surjective : forall x, { y | (tretract_g I) y = Some x }.
+  Proof. intros x. pose proof (tretract_g_adjoint x). eauto. Defined.
+
+  Lemma tretract_f_injective : forall x1 x2, tretract_f I x1 = tretract_f I x2 -> x1 = x2.
+  Proof.
+    intros x1 x2 H. enough (Some x1 = Some x2) as HE by now inv HE.
+    erewrite <- !tretract_g_adjoint; eauto. now rewrite H.
+  Qed.
+    
+End TightRetract.
 
 
 Section Retract_Compose.
@@ -36,25 +80,42 @@ Section Retract_Compose.
   Definition retract_comp_g :=
     fun z =>
       match retract_g inj2 z with
-      | Some y =>retract_g inj1 y
+      | Some y => retract_g inj1 y
       | None => None
       end.
 
-  Lemma retract_comp_inv : forall (x : X), retract_comp_g (retract_comp_f (x)) = Some x.
+  Lemma retract_comp_adjoint : forall (x : X), retract_comp_g (retract_comp_f (x)) = Some x.
   Proof.
     unfold retract_comp_f, retract_comp_g. intros x. now do 2 rewrite retract_g_adjoint.
   Qed.
 
-  Hypothesis (tight1 : retract_tight inj1) (tight2 : retract_tight inj2).
+  Definition retract_compse := Build_retract retract_comp_adjoint.
 
-  Definition retract_compose : retract X Z := Build_retract retract_comp_inv.
-
-  Lemma retract_comp_tight : retract_tight retract_compose.
-  Proof.
-    hnf. intros x y H. unfold retract_compose in *. cbn in *. unfold retract_comp_g, retract_comp_f in *.
-    destruct (retract_g inj2 y) eqn:E.
-    - apply tight2 in E as ->. apply tight1 in H as ->. reflexivity.
-    - congruence.
-  Qed.
-  
 End Retract_Compose.
+
+Section TightRetract_Compose.
+
+  Variable (X Y Z : Type).
+  Hypothesis (inj1 : tight_retract X Y) (inj2 : tight_retract Y Z).
+
+  Definition tretract_comp_f := fun x => tretract_f inj2 (tretract_f inj1 x).
+
+  Definition tretract_comp_g :=
+    fun z =>
+      match tretract_g inj2 z with
+      | Some y => tretract_g inj1 y
+      | None => None
+      end.
+
+  Lemma tretract_comp_inv : forall x z, tretract_comp_g z = Some x <-> z = tretract_comp_f x.
+  Proof.
+    unfold tretract_comp_f, tretract_comp_g. intros x z. split.
+    - intros H. destruct (tretract_g inj2 z) eqn:E.
+      + apply tretract_inv in E as ->. apply tretract_inv in H as ->. reflexivity.
+      + congruence.
+    - intros ->. now do 2 rewrite tretract_g_adjoint.
+  Qed.
+
+  Definition tretract_compose := Build_tight_retract tretract_comp_inv.
+
+End TightRetract_Compose.
